\documentclass{article}
\usepackage[margin=0.75in]{geometry}
\usepackage{amsmath}
\usepackage{amssymb}
\usepackage{graphicx}
\usepackage[thinc]{esdiff}
\usepackage{cancel}
\usepackage{titlesec}
\setlength{\parindent}{0em}

\begin{document}

\Large{
    Given, $x$ and $y$ are independent random vaiables. \\
    To be proved: $var (x-y) = var(x) + var(y)$\\
    We know $var(x) = E(x^2)-\mu^2$\\
    at $E(x),\;\mu_1$ and $E(y),\;\mu_2$\\
    \begin{eqnarray*}
        L.S: var(x-y) &=& E\left\{(x-y)^2\right\} -\left[E(x-y)\right]^2\\
        &=& E\left\{x^2-2xy+y^2\right\}-\left[E(x)-E(y)\right]^2\\
        &=& E(x^2) - 2E(xy) + E(y^2)- [\mu_1 - \mu_2]^2\\
        && \hspace{3cm}\text{[substituting $E(x),\;\mu_1$ and $E(y),\;\mu_2$]}\\
        &=& E(x^2) - 2E(x)\cdot E(y)+ E(y^2)-\left(\mu_1^2 - 2\mu_1\mu_2 + \mu_2^2\right)\\
        && \hspace{3cm}\text{[using $E(xy)=E(x).E(y)$]}\\
        &=& E(x^2)-2\mu_1\mu_2+E(y^2)-\mu_1^2+2\mu_1\mu_2 -\mu_2^2\\
        && \hspace{3cm}\text{[using $E(x)=\mu_1$ and $E(y)= \mu_2$]}\\
        &=& E(x^2)-\mu_1^2+E(y^2)-\mu_2^2\\
        &=& var(x)+var(y) \hspace{1cm}\text{[from variance formula]}\\
        &=& R.S
    \end{eqnarray*}

$\therefore var(x-y) = var(x) + var(y)$\\

\hspace{7cm}[Proved]

}
\end{document}
